BubbleSort

BubbleSort.dfy
@@ -1,25 +1,44 @@
+predicate sorted_range(a: array<int>, l:nat, u:nat)
+  requires a != null;
+  requires 0 <= l <= u <= a.Length;
+  reads a;
+{
+  forall i, j :: l <= i < j < u ==> a[i] <= a[j]
+}
+predicate pivot(a:array<int>, pv:nat, l:nat, up:nat)
+  requires a != null;
+  requires 0 <= l <= pv <= up <= a.Length;
+  reads a;
+{
+  forall u , v :: l <= u < pv < v < up ==> a[u] <= a[v]
+}
+
 /* see visualgo for an animation of Bubble sort */
 method bubbleSort (a: array<int>)
   requires a != null && a.Length > 1;
-  ensures forall u, v :: 0 <= u < v < a.Length ==> a[u] <= a[v];
+  ensures sorted_range(a, 0, a.Length);
+  ensures multiset(a[..]) == multiset(old(a[..]));
   modifies a;
 {
   var i:nat := 1;
   while (i < a.Length)
     invariant i <= a.Length;
-    invariant forall u, v:: 0 <= u < v < i ==> a[u] <= a[v];
+    invariant sorted_range (a, 0, i);
+    invariant multiset(a[..]) == multiset(old(a[..]));
   {
     var j:nat := i;
     while (j > 0)
       invariant 0 <= j <= i;
-      invariant forall u, v :: 0 <= u < v < j ==> a[u] <= a[v];
-      invariant forall u, v :: j <= u < v < i+1 ==> a[u] <= a[v];
-      invariant forall u , v :: 0 <= u < j < v < i+1 ==> a[u] <= a[v]
+      invariant sorted_range (a, 0, j)
+      invariant sorted_range (a, j, i+1);
+      invariant pivot(a, j, 0, i+1);
+      invariant multiset(a[..]) == multiset(old(a[..]));
     {
       if (a[j-1] > a[j]) {
         var temp:int := a[j-1];
-        a[j] := temp;
         a[j-1] := a[j];
+        a[j] := temp;
+
       }
       j := j - 1;
     }
